Updates

generic/Zeta.Generic.Global.fst
@@ -1,13 +1,6 @@
 module Zeta.Generic.Global
 
-let add_set
-  (#vspec: verifier_spec)
-  (ep: epoch)
-  (gl: verifiable_log vspec): mset_ms_hashfn_dom vspec.app
-  = admit()
 
-let evict_set
-  (#vspec: verifier_spec)
-  (ep: epoch)
-  (gl: verifiable_log vspec): mset_ms_hashfn_dom vspec.app
+let to_fm (#vspec: verifier_spec) (#b:eqtype) (#pred:_) (p:nat) (tfn: cond_idxfn_t #vspec b pred)
+  : ssfm_t (verifier_log_entry vspec) b p
   = admit()
