generic/Zeta.Generic.Global.fsti
@@ -31,24 +31,36 @@ let verifiable #vspec (gl: vlog vspec) =
 
 let verifiable_log vspec = gl:vlog vspec {verifiable gl}
 
-let clock #vspec (gl: verifiable_log vspec) (i: sseq_index gl) =
-  let tid, i' = i in
-  let tl = thread_log gl tid in
-  T.clock tl i'
+let idxfn #vspec (#b:eqtype) (tfn: idxfn_t vspec b) (gl: verifiable_log vspec) (ti: sseq_index gl): b
+  = let t,i = ti in
+    let tl = thread_log gl t in
+    tfn tl i
 
+let clock #vspec = idxfn (T.clock #vspec)
+
+(* given a conditional thread index function (e.g., blum_evict_elem) we can construct a filter-map pred *)
+val to_fm (#vspec: verifier_spec) (#b:eqtype) (#pred:_) (p:nat) (tfn: cond_idxfn_t #vspec b pred)
+  : ssfm_t (verifier_log_entry vspec) b p
 
 (* blum add set elements for a given epoch *)
 let add_set
   (#vspec: verifier_spec)
   (ep: epoch)
   (gl: verifiable_log vspec): mset_ms_hashfn_dom vspec.app
-  = admit()
+  = let open Zeta.MultiSet.SSeq in
+    (* filter map specification that filter by AddB? and maps them to blum add elem *)
+    let fm = to_fm (S.length gl) (T.blum_add_elem #vspec #ep) in
+    (* get a seq of seq of blum-add-elems and convert them to multiset *)
+    sseq2mset (ssfilter_map fm gl)
 
 (* blum evict set elements for a given epoch *)
-val evict_set
+let evict_set
   (#vspec: verifier_spec)
   (ep: epoch)
   (gl: verifiable_log vspec): mset_ms_hashfn_dom vspec.app
+  = let open Zeta.MultiSet.SSeq in
+    let fm = to_fm (S.length gl) (T.blum_evict_elem #vspec #ep) in
+    sseq2mset (ssfilter_map fm gl)
 
 (* verifiable log property that add- and evict sets are the same *)
 let aems_equal_for_epoch #vspec
@@ -71,3 +83,10 @@ let aems_equal_upto #vspec (epmax: epoch) (gl: verifiable_log vspec) =
 (* global log whose add and evict multisets are equal *)
 let ms_verifiable_log #vspec (ep: epoch)
   = gl:verifiable_log vspec{aems_equal_upto ep gl}
+
+(* filter-mapped sequence of sequence app-function-call results *)
+let appfn_call_res
+  (#vspec: verifier_spec)
+  (gl: verifiable_log vspec): sseq (Zeta.AppSimulate.appfn_call_res vspec.app)
+  = let fm = to_fm (S.length gl) (T.appfn_call_res #vspec) in
+    ssfilter_map fm gl
