generic/Zeta.Generic.Thread.fsti
@@ -41,15 +41,18 @@ val verifiable_implies_prefix_verifiable (#vspec:verifier_spec)
         [SMTPat (prefix tl i)]
 
 (* the verifier state after processing i entries *)
-let state_at #vspec (tl: verifiable_log vspec) (i:nat{i <= length tl}) =
+let state_pre #vspec (tl: verifiable_log vspec) (i:nat{i <= length tl}) =
   (verify (prefix tl i))
+
+let state_post #vspec (tl: verifiable_log vspec) (i:seq_index tl)
+  = (verify (prefix tl (i+1)))
 
 (* the state after processing i'th entry is obtained by applying the verify
  * step to the state before processing the i'th entry *)
 val lemma_state_transition (#vspec:verifier_spec) (tl: verifiable_log vspec) (i: seq_index tl):
-  Lemma (ensures (state_at tl (i + 1) ==
-                  verify_step (index tl i) (state_at tl i)))
-        [SMTPat (verify_step (index tl i) (state_at tl i))]
+  Lemma (ensures (state_post tl i ==
+                  verify_step (index tl i) (state_pre tl i)))
+        [SMTPat (verify_step (index tl i) (state_pre tl i))]
 
 (* the type of functions that return a value at position i *)
 let idxfn_t_base (vspec: verifier_spec) (b: eqtype)
@@ -71,6 +74,7 @@ let cond_idxfn_t_base #vspec (b:eqtype) (f: idxfn_t vspec bool)
 
 let cond_prefix_property #vspec #b (#f: idxfn_t vspec bool) (m: cond_idxfn_t_base b f)
   = forall (tl: verifiable_log vspec) (i:nat) (j:nat).
+      {:pattern m (prefix tl j) i}
       j <= length tl ==>
       i < j ==>
       f tl i ==>
@@ -103,4 +107,13 @@ val blum_add_elem (#vspec:_) (#ep: epoch):
 val is_blum_evict (#vspec:_) (ep: epoch): idxfn_t vspec bool
 
 val blum_evict_elem (#vspec:_) (#ep: epoch):
-  cond_idxfn_t #vspec (ms_hashfn_dom vspec.app) (is_blum_add ep)
+  cond_idxfn_t #vspec (ms_hashfn_dom vspec.app) (is_blum_evict ep)
+
+(* is the i'th entry an app function *)
+val is_appfn (#vspec:_): idxfn_t vspec bool
+
+open Zeta.AppSimulate
+
+(* for an appfn entry, return the function call params and result *)
+val appfn_call_res (#vspec:_):
+  cond_idxfn_t #vspec (appfn_call_res vspec.app) is_appfn
