generic/Zeta.GenericVerifier.fsti
@@ -1,6 +1,7 @@
 module Zeta.GenericVerifier
 
 open Zeta.App
+open Zeta.AppSimulate
 open Zeta.Time
 open Zeta.MultiSetHashDomain
 open Zeta.Record
@@ -103,16 +104,43 @@ let is_evict #vspec (e: verifier_log_entry vspec): bool =
   | EvictBM _ _ _ -> true
   | _ -> false
 
+let evict_slot #vspec (e: verifier_log_entry vspec{is_evict e})
+  = match e with
+    | EvictM s _ -> s
+    | EvictB s _ -> s
+    | EvictBM s _ _ -> s
+
 let is_blum_evict #vspec (e: verifier_log_entry vspec) =
   match e with
   | EvictB _ _ -> true
   | EvictBM _ _ _ -> true
   | _ -> false
 
+let blum_evict_timestamp #vspec (e: verifier_log_entry vspec {is_blum_evict e})
+  = match e with
+    | EvictB _ t -> t
+    | EvictBM _ _ t -> t
+
 let is_merkle_evict #vspec (e:verifier_log_entry vspec): bool =
   match e with
   | EvictM _ _ -> true
   | _ -> false
+
+let is_add #vspec (e: verifier_log_entry vspec)
+  = match e with
+    | AddM _ _ _ -> true
+    | AddB _ _ _ _ -> true
+    | _ -> false
+
+let add_record #vspec (e: verifier_log_entry vspec {is_add e})
+  = match e with
+    | AddM r _ _ -> r
+    | AddB r _ _ _ -> r
+
+let add_slot #vspec (e: verifier_log_entry vspec {is_add e})
+  = match e with
+    | AddM _ s _ -> s
+    | AddB _ s _ _ -> s
 
 val get_record_set (#vspec: verifier_spec_base) (ss: S.seq (vspec.slot_t)) (vtls: vspec.vtls_t {vspec.valid vtls}):
   (let record_t = app_record vspec.app.adm in
@@ -162,6 +190,18 @@ let verify_step (#vspec: verifier_spec_base)
         (* update the verifier store with the writes of the function *)
         else update_record_set ss vtls ws
 
+let appfn_result #vspec
+  (e: verifier_log_entry vspec{is_appfn e})
+  (vtls: vspec.vtls_t {vspec.valid (verify_step e vtls)})
+  : appfn_call_res vspec.app
+  = assert(vspec.valid vtls);
+    match e with
+    | RunApp f p ss ->
+      let fn = appfn f in
+      let rs = Some?.v (get_record_set ss vtls) in
+      let _,o,_ = fn p rs in
+      {fid_cr = f; arg_cr = p; inp_cr = rs; res_cr = o}
+
 let verifier_failure_propagating (#vspec: _) (e: verifier_log_entry vspec) (vtls: vspec.vtls_t):
   Lemma (requires (vspec.valid (verify_step e vtls)))
         (ensures (vspec.valid vtls)) = ()
@@ -183,6 +223,26 @@ let thread_id_constant_prop (vspec: verifier_spec_base) =
     let tid_post = vspec.tid (verify_step e vtls) in
     tid_pre = tid_post
 
+(* a slot is non-empty before evict and empty after, if the verify succeeds *)
+let evict_prop (vspec: verifier_spec_base) =
+  forall (e: verifier_log_entry vspec) (vtls: vspec.vtls_t).
+    {:pattern verify_step e vtls}
+    let vtls' = verify_step e vtls in
+    is_evict e ==>
+    vspec.valid vtls' ==>
+    Some? (vspec.get (evict_slot e) vtls) /\
+    None? (vspec.get (evict_slot e) vtls')
+
+(* a slot is empty before add and non-empty after, if the add succeeds *)
+let add_prop (vspec: verifier_spec_base) =
+  forall (e: verifier_log_entry vspec) (vtls: vspec.vtls_t).
+    {:pattern verify_step e vtls}
+    let vtls' = verify_step e vtls in
+    is_add e ==>
+    vspec.valid vtls' ==>
+    None? (vspec.get (add_slot e) vtls) /\
+    Some? (vspec.get (add_slot e) vtls')
+
 let verifier_log vspec = S.seq (verifier_log_entry vspec)
 
 let rec verify #vspec (tid: thread_id) (l: verifier_log vspec):
@@ -194,4 +254,5 @@ let rec verify #vspec (tid: thread_id) (l: verifier_log vspec):
     let vtls' = verify tid (SA.prefix l (n-1)) in
     verify_step (S.index l (n-1)) vtls'
 
-let verifier_spec = vspec:verifier_spec_base {clock_monotonic_prop vspec /\ thread_id_constant_prop vspec}
+let verifier_spec = vspec:verifier_spec_base
+    {clock_monotonic_prop vspec /\ thread_id_constant_prop vspec /\ evict_prop vspec /\ add_prop vspec}
